backend/Constpropproof.v
@@ -43,7 +43,9 @@ Hypothesis SEVALID: Genv.valid_for (erase_program prog) se.
 
 Let ge := Genv.globalenv se prog.
 Let tge := Genv.globalenv tse tprog.
-
+Let gs := Genv.genv_sup se.
+Let tgs := Genv.genv_sup tse.
+                        
 (** * Correctness of the code transformation *)
 
 (** We now show that the transformed code after constant propagation
@@ -326,7 +328,7 @@ Inductive match_stackframes (j: meminj): stackframe -> stackframe -> Prop :=
         (Stackframe res (transf_function (romem_for prog) f) (Vptr sp' Ptrofs.zero) pc rs').
 
 Definition m01 := match w with
-                 | injpw f m1 m2 Hm => m1
+                 | injpw f _ _ m1 m2 Hm => m1
                  end.
 
 Inductive match_states: nat -> state -> state -> Prop :=
@@ -336,7 +338,7 @@ Inductive match_states: nat -> state -> state -> Prop :=
            (PC: match_pc f rs m n pc pc')
            (REGS: regset_inject j rs rs')
            (SP: j sp = Some (sp',0))
-           (INCR: injp_acc w (injpw j m m' MEM))
+           (INCR: injp_acc w (injpw j gs tgs m m' MEM))
            (RO: ro_acc m01 m),
       match_states n (State s f (Vptr sp Ptrofs.zero) pc rs m)
                     (State s' (transf_function (romem_for prog) f) (Vptr sp' Ptrofs.zero) pc' rs' m')
@@ -345,7 +347,7 @@ Inductive match_states: nat -> state -> state -> Prop :=
            (STACKS: list_forall2 (match_stackframes j) s s')
            (VF: Val.inject j vf vf')
            (ARGS: Val.inject_list j args args')
-           (INCR: injp_acc w (injpw j m m' MEM))
+           (INCR: injp_acc w (injpw j gs tgs m m' MEM))
            (RO: ro_acc m01 m),
       match_states O (Callstate s vf args m)
                      (Callstate s' vf' args' m')
@@ -353,7 +355,7 @@ Inductive match_states: nat -> state -> state -> Prop :=
       forall s v m s' v' m' j MEM
            (STACKS: list_forall2 (match_stackframes j) s s')
            (RES: Val.inject j v v')
-           (INCR: injp_acc w (injpw j m m' MEM))
+           (INCR: injp_acc w (injpw j gs tgs m m' MEM))
            (RO: ro_acc m01 m),
       match_states O (Returnstate s v m)
                      (Returnstate s' v' m').
@@ -364,7 +366,7 @@ Lemma match_states_succ:
   regset_inject j rs rs' ->
   Mem.inject j m m' ->
   j sp = Some (sp',0) ->
-  injp_acc w (injpw j m m' MEM) ->
+  injp_acc w (injpw j gs tgs m m' MEM) ->
   ro_acc m01 m ->
   match_states O (State s f (Vptr sp Ptrofs.zero) pc rs m)
                  (State s' (transf_function (romem_for prog) f) (Vptr sp' Ptrofs.zero) pc rs' m').
@@ -381,7 +383,7 @@ Proof.
 Qed.
 
 Lemma match_stbls_incr : forall j m1 m2 MEM,
-    injp_acc w (injpw j m1 m2 MEM) ->
+    injp_acc w (injpw j gs tgs m1 m2 MEM) ->
     Genv.match_stbls j ge tge.
 Proof.
   intros.
@@ -524,7 +526,7 @@ Proof.
   exploit Mem.storev_mapped_inject. eauto. eauto.
   eapply Mem.val_lessdef_inject_compose; eauto. apply REGS.
   intros (m2' & X & Y).
-  assert (INCR0: injp_acc (injpw j m m'0 MEM) (injpw j m' m2' Y)).
+  assert (INCR0: injp_acc (injpw j gs tgs m m'0 MEM) (injpw j gs tgs m' m2' Y)).
   eapply injp_acc_storev; eauto.
   eapply Mem.val_lessdef_inject_compose; eauto.
   left; econstructor; econstructor; split.
@@ -555,7 +557,7 @@ Proof.
   exploit (ros_address_translated j ros); eauto. intros FEXT.
   exploit functions_translated; eauto using ros_address_translated. intro FIND.
   TransfInstr; intro.
-  assert (INCR0 : injp_acc (injpw j m m'0 MEM) (injpw j m' m2' B)).
+  assert (INCR0 : injp_acc (injpw j gs tgs m m'0 MEM) (injpw j gs tgs m' m2' B)).
   eapply injp_acc_free with (lo1 := 0); eauto.
   replace (0+0) with 0 by lia.
   replace (0 + fn_stacksize f + 0) with (fn_stacksize f) by lia. eauto.
@@ -597,6 +599,8 @@ Opaque builtin_strength_reduction.
     red. eauto using external_call_readonly.
     red. intros. eapply external_call_max_perm; eauto.
     red. intros. eapply external_call_max_perm; eauto.
+    eapply Mem.unchanged_on_implies. eauto. intros b ofs [X Y] Z. eauto.
+    eapply Mem.unchanged_on_implies. eauto. intros b ofs [X Y] Z. eauto.
     unfold m01 in *. inv INCR. eapply ro_acc_trans. eauto.
     eapply ro_acc_external; eauto.
   }
@@ -655,7 +659,7 @@ Opaque builtin_strength_reduction.
 
 - (* Ireturn *)
   exploit Mem.free_parallel_inject; eauto. intros [m2' [A B]]. simpl in A. rewrite Z.add_0_r in A.
-  assert (INCR0 : injp_acc (injpw j m m'0 MEM) (injpw j m' m2' B)).
+  assert (INCR0 : injp_acc (injpw j gs tgs m m'0 MEM) (injpw j gs tgs m' m2' B)).
   eapply injp_acc_free with (lo1 := 0); eauto.
   replace (0+0) with 0 by lia.
   replace (0 + fn_stacksize f + 0) with (fn_stacksize f) by lia. eauto.
@@ -672,7 +676,7 @@ Opaque builtin_strength_reduction.
   exploit Mem.alloc_parallel_inject. eauto. eauto. apply Z.le_refl. apply Z.le_refl.
   intros (f' & m2' & b2 & A & B & C & D & E).
   simpl. unfold transf_function.
-  assert (INCR0 :injp_acc (injpw j m m'0 MEM) (injpw f' m' m2' B)).
+  assert (INCR0 :injp_acc (injpw j gs tgs m m'0 MEM) (injpw f' gs tgs m' m2' B)).
   eapply injp_acc_alloc; eauto.
   left; exists O; econstructor; split.
   eapply exec_function_internal; simpl; eauto.
@@ -697,6 +701,8 @@ Opaque builtin_strength_reduction.
   red. eauto using external_call_readonly.
   red. intros. eapply external_call_max_perm; eauto.
   red. intros. eapply external_call_max_perm; eauto.
+  eapply Mem.unchanged_on_implies. eauto. intros b ofs [X Y] Z. eauto.
+  eapply Mem.unchanged_on_implies. eauto. intros b ofs [X Y] Z. eauto.
   eapply ro_acc_trans. eauto. constructor.
   red. intros. eapply external_call_readonly; eauto.
   eapply external_call_support; eauto.
@@ -723,7 +729,7 @@ Proof.
   - setoid_rewrite <- (sig_function_translated (romem_for prog) (Internal f)).
     constructor; auto.
   - rewrite <- H0 in *. cbn in *. econstructor. 
-    4: { instantiate (1:= Hm). rewrite <- H0. reflexivity. }
+    4: { instantiate (1:= Hm). rewrite <- H0. inv GE.  reflexivity. }
     all : eauto. constructor.
     eapply ro_acc_refl.
   - rewrite <- H0 in *. cbn in *. eapply sound_memory_ro_sound_state; eauto.
@@ -739,10 +745,27 @@ Proof.
   exists (cr v' m'). split. constructor; eauto.  
   eexists; split. constructor; eauto.
   constructor; eauto.
+
   eexists ; split; eauto. econstructor; eauto.
   econstructor; eauto.
 Qed.
 
+Lemma BCinvalid_not_global : forall j b1 b2 se1 se2 (bc: block_classification) delta,
+    j b1 = Some (b2 ,delta) ->
+    bc b1 = BCinvalid ->
+    genv_match bc se1 ->
+    Genv.match_stbls j se1 se2 ->
+    ~ sup_In b1 (Genv.genv_sup se1) /\ ~ sup_In b2 (Genv.genv_sup se2). 
+Proof.
+  intros.
+  destruct H1 as [X Y].
+  assert (~ sup_In b1 (Genv.genv_sup se1)).
+  intro. exploit Y; eauto.
+  intros [A B]. congruence.
+  split. eauto.
+  intro. apply H1. eapply Genv.mge_separated; eauto.
+Qed.
+              
 Lemma transf_external_states:
   forall n st1 st2 q1, match_states n st1 st2 -> sound_state prog ge st1 -> at_external ge st1 q1 ->
   exists w' q2, at_external tge st2 q2 /\ match_query (ro @ cc_c injp) w' q1 q2 /\ match_senv (ro @ cc_c injp) w' se tse /\
@@ -766,7 +789,7 @@ Proof.
     destruct (bc b); simpl; eauto;
     destruct (j b) as [[x y]|]; eauto.
   }
-  eexists (se,(row se m),(injpw _ _ _ MEM')). eexists. cbn. intuition idtac.
+  eexists (se,(row se m),(injpw _ _ _ _ _ MEM')). eexists. cbn. intuition idtac.
   - econstructor; eauto.
   - assert (sound_memory_ro ge m).
     {
@@ -781,7 +804,7 @@ Proof.
       split. intro. congruence. intro. apply H in H1.
       apply Genv.find_invert_symbol in H1. cbn in *. congruence.
       inv GE. rewrite <- H4 in INCR.
-      inversion INCR. inversion H15. eauto.
+      inversion INCR. inversion H17. eauto.
     }
     eexists. split. constructor. constructor; eauto.
     econstructor; eauto.
@@ -801,9 +824,9 @@ Proof.
     eapply Genv.match_stbls_compose.
     eapply inj_of_bc_preserves_globals; eauto.
     apply MSTB.
-    inversion H15. eauto. inversion H16. eauto.
+    inversion H17. eauto. inversion H18. eauto.
   - inv H2. destruct H1 as (r3 & Hr1& Hr2). inv Hr1. inv H1. rename H3 into ROACC.
-    destruct Hr2 as ([j' s1 s2 MEM''] & Hw' & Hr).
+    destruct Hr2 as ([j' gs1 gs2 s1 s2 MEM''] & Hw' & Hr).
     inv Hw'.
     inv Hr. cbn in *. inv H5. simpl in *.
     eexists _, (Returnstate s' vres2 m2'); split.
@@ -819,7 +842,7 @@ Proof.
       { red. intros. destruct (block_class_eq (bc b) BCinvalid).
         unfold j''; rewrite e; eauto. rewrite H1.
         reflexivity.
-        unfold j''. destruct (bc b) eqn:BC; try congruence; apply H13;
+        unfold j''. destruct (bc b) eqn:BC; try congruence; apply H17;
         unfold compose_meminj, inj_of_bc;
         rewrite BC, H1; reflexivity.
       }
@@ -828,14 +851,15 @@ Proof.
         destruct (bc b) eqn:BC;
           unfold j''; rewrite BC; eauto.
         destruct (j b) as [[b'' d']|] eqn :Hj.
-        exploit H14; eauto. unfold compose_meminj, inj_of_bc.
+        exploit H18; eauto. unfold compose_meminj, inj_of_bc.
         rewrite BC. reflexivity. intros [A B].
         inversion MEM. exploit mi_freeblocks; eauto. intro. congruence.
         eauto.
       }
       assert(MEM''' : Mem.inject j'' m'0 m2').
       {
-       clear - JBC_COMPOSE MEM MEM'' INCR1 INCR2 H7 H8 H9 H10 H11 H12 H13 H14.
+        exploit match_stbls_incr; eauto. intro MSTBL.
+        clear - JBC_COMPOSE MEM MEM'' MSTBL GE0 INCR1 INCR2 H10 H12 H13 H14 H15 H16 H17 H18.
         assert (j''_INV: forall b b' d, j'' b = Some (b',d) -> (j' b = Some (b',d)) \/
                                                            (j b = Some (b',d) /\ bc b = BCinvalid)).
         {
@@ -847,10 +871,10 @@ Proof.
         {
           intros. destruct (jbc b) as [[b'' d']|] eqn:Hjbc.
           right.
-          rewrite <- JBC_COMPOSE in Hjbc. erewrite H13 in H; eauto. inv H.
+          rewrite <- JBC_COMPOSE in Hjbc. erewrite H17 in H; eauto. inv H.
           rewrite JBC_COMPOSE in Hjbc.  unfold jbc in Hjbc.
           destruct (bc b); try congruence; split; try congruence; eauto.
-          left. exploit H14; eauto. rewrite JBC_COMPOSE. eauto.
+          left. exploit H18; eauto. rewrite JBC_COMPOSE. eauto.
           intros [A B]. eauto.
         }
         inv MEM''.
@@ -877,44 +901,49 @@ Proof.
         -- inv mi_inj. constructor; eauto.
            ++ intros. destruct (bc b1) eqn:BC;
               unfold j'' in H; rewrite BC in H; eauto.
-              destruct (j b1) as [[b2' d']|] eqn:Hjb1; eauto.
+              destruct (j b1) as [[b2' d']|] eqn:Hjb1; eauto. inv H.
+              exploit BCinvalid_not_global; eauto. intros [STK1 STK2].
               assert (P1: Mem.perm m b1 ofs k p).
               {
-                inversion H11. apply unchanged_on_perm; eauto.
+                inversion H15. apply unchanged_on_perm; eauto.
                 inv MEM. destruct (Mem.sup_dec b1 (Mem.support m)).
                 eauto. exploit mi_freeblocks0; eauto. congruence.
               }
-              inv H. inversion H12. eapply unchanged_on_perm; eauto.
+              inversion H16. eapply unchanged_on_perm; eauto.
               inv MEM. eauto.
               eapply Mem.perm_inject; eauto.
            ++ intros. destruct (bc b1) eqn:BC; unfold j'' in H; rewrite BC in H; eauto.
               destruct (j b1) as [[b2' d']|] eqn:Hjb1; eauto.
-              inv H. inversion MEM. inv mi_inj. eapply mi_align0; eauto.
+              inv H.
+              exploit BCinvalid_not_global; eauto. intros [STK1 STK2].
+              inversion MEM. inv mi_inj. eapply mi_align0; eauto.
               red. intros. exploit H0; eauto.
-              intro. inv H11. eapply unchanged_on_perm; eauto with mem.
+              intro. inv H15. eapply unchanged_on_perm; eauto with mem.
               eapply Mem.valid_block_inject_1; eauto.
            ++ intros. destruct (bc b1) eqn:BC; unfold j'' in H; rewrite BC in H.
               destruct (j b1) as [[b2' d']|] eqn:Hjb1; eauto.
               inv H.
+              exploit BCinvalid_not_global; eauto. intros [STK1 STK2].
               assert (P1: Mem.perm m b1 ofs Cur Readable).
               {
-                inversion H11. apply unchanged_on_perm; eauto.
+                inversion H15. apply unchanged_on_perm; eauto.
                 inv MEM. destruct (Mem.sup_dec b1 (Mem.support m)).
                 eauto. exploit mi_freeblocks0; eauto. congruence.
               }
               erewrite Mem.unchanged_on_contents; eauto.
-              inv H12.
+              inv H16.
               rewrite unchanged_on_contents; eauto.
-              2: eapply Mem.perm_inject; eauto. inv MEM. inv mi_inj.
+              2:{ eapply Mem.perm_inject; eauto. }   inv MEM. inv mi_inj.
+              eapply memval_inject_incr; eauto. split; eauto.
               all: (eapply memval_inject_incr; eauto).
         -- (* source_range *)
           intros. unfold j''. destruct (bc b); eauto.
           destruct (j b) as [[b' d']|] eqn:Hjb; eauto.
-          inv H11. exploit Mem.valid_block_inject_1; eauto. intro.
+          inv H15. exploit Mem.valid_block_inject_1; eauto. intro.
           exfalso. apply H. eapply unchanged_on_support; eauto.
         -- intros. unfold j'' in H. destruct (bc b); eauto.
            destruct (j b) as [[b'' d']|] eqn:Hjb; eauto. inv H.
-           inv H12. exploit Mem.valid_block_inject_2; eauto. intro.
+           inv H16. exploit Mem.valid_block_inject_2; eauto. intro.
            eapply unchanged_on_support; eauto.
         -- red. intros.
            destruct (j''_INV _ _ _ H0) as [A|[A1 A2]];
@@ -922,27 +951,28 @@ Proof.
            ++ destruct (j'_INV _ _ _ A) as [C|[C1 C2]]; eauto.
               left. exploit Mem.valid_block_inject_2; eauto. intro. congruence.
               inversion MEM. eapply mi_no_overlap0; eauto.
-              eapply H9; eauto. eapply Mem.valid_block_inject_1; eauto.
-              eapply H9; eauto. eapply Mem.valid_block_inject_1; eauto.
+              eapply H13; eauto. eapply Mem.valid_block_inject_1; eauto.
+              eapply H13; eauto. eapply Mem.valid_block_inject_1; eauto.
            ++ destruct (j'_INV _ _ _ B) as [C|[C1 C2]]; eauto.
               left. exploit Mem.valid_block_inject_2. apply A1. eauto. intro. congruence.
               inversion MEM. eapply mi_no_overlap0; eauto.
-              eapply H9; eauto. eapply Mem.valid_block_inject_1; eauto.
-              eapply H9; eauto. eapply Mem.valid_block_inject_1; eauto.
+              eapply H13; eauto. eapply Mem.valid_block_inject_1; eauto.
+              eapply H13; eauto. eapply Mem.valid_block_inject_1; eauto.
            ++ inversion MEM. eapply mi_no_overlap0; eauto.
-              eapply H9; eauto. eapply Mem.valid_block_inject_1; eauto.
-              eapply H9; eauto. eapply Mem.valid_block_inject_1; eauto.
+              eapply H13; eauto. eapply Mem.valid_block_inject_1; eauto.
+              eapply H13; eauto. eapply Mem.valid_block_inject_1; eauto.
         -- intros. destruct (j''_INV _ _ _ H) as [A|[A1 A2]]; eauto.
            inversion MEM. eapply mi_representable0; eauto.
-           destruct H0. left. eapply H9; eauto. eapply Mem.valid_block_inject_1; eauto.
-           right. eapply H9; eauto. eapply Mem.valid_block_inject_1; eauto.
+           destruct H0. left. eapply H13; eauto. eapply Mem.valid_block_inject_1; eauto.
+           right. eapply H13; eauto. eapply Mem.valid_block_inject_1; eauto.
         -- intros. destruct (j''_INV _ _ _ H) as [A|[A1 A2]]; eauto.
+           exploit BCinvalid_not_global; eauto. intros [STK1 STK2].
            destruct (Mem.perm_dec m'0 b1 ofs Max Nonempty); eauto.
-           apply H9 in p0. left.
+           apply H13 in p0. left.
            inversion MEM. exploit mi_perm_inv0; eauto.
-           inv H12. eapply unchanged_on_perm; eauto.
+           inv H16. eapply unchanged_on_perm; eauto.
            intros [A|B].
-           inv H11. eapply unchanged_on_perm; eauto with mem. congruence.
+           inv H15. eapply unchanged_on_perm; eauto with mem. congruence.
            eapply Mem.valid_block_inject_1; eauto. 
       }
       econstructor.
@@ -951,15 +981,15 @@ Proof.
       * eauto.
       * etransitivity; eauto. instantiate (1:= MEM'''). econstructor; eauto.
         eapply Mem.unchanged_on_implies; eauto.
-        intros. red. red in H1. unfold compose_meminj, inj_of_bc.
+        intros. destruct H1. split; eauto. red. red in H1. unfold compose_meminj, inj_of_bc.
         destruct (bc b); simpl; try (rewrite H1); eauto.
         eapply Mem.unchanged_on_implies; eauto.
-        intros. red. red in H1. intros. eapply H1; eauto.
-        unfold compose_meminj,inj_of_bc in H4.
-        destruct (bc b0); simpl in H4; try congruence;
+        intros. destruct H1. split; eauto. red. red in H1. intros. eapply H1; eauto.
+        unfold compose_meminj,inj_of_bc in H5.
+        destruct (bc b0); simpl in H5; try congruence;
         destruct (j b0) as [[b1 d1]|]; eauto.
         red. intros.
-        eapply H14; eauto. unfold compose_meminj, inj_of_bc.
+        eapply H18; eauto. unfold compose_meminj, inj_of_bc.
         destruct (bc b1) eqn:BC; try (rewrite H1; reflexivity). reflexivity.
         unfold j'' in H2.
         destruct (bc b1) eqn:BC; eauto. rewrite H1 in H2. eauto.
@@ -970,9 +1000,9 @@ Proof.
       {
         intros. destruct (jbc b) as [[b' delta] | ] eqn:EQ.
         rewrite <- JBC_COMPOSE in EQ.
-        eapply H13; eauto.
+        eapply H17; eauto.
         destruct (j' b) as [[b'' delta'] | ] eqn:EQ'; auto.
-        exploit H14; eauto. rewrite JBC_COMPOSE. eauto.
+        exploit H18; eauto. rewrite JBC_COMPOSE. eauto.
         intros [A B]. exfalso. eauto.
       }
       set (f := fun b => if Mem.sup_dec b (Mem.support m)
@@ -1033,30 +1063,33 @@ Proof.
       inv MM. exploit mmatch_top. eauto.
       intros [D E]. eapply D; eauto.
       erewrite Mem.load_unchanged_on_1 in H2; eauto.
-      intros. red. unfold compose_meminj, inj_of_bc.
+      intros. split. red. unfold compose_meminj, inj_of_bc.
       destruct (bc b); try congruence. rewrite B. reflexivity.
       rewrite B. reflexivity. rewrite B. reflexivity.
+      intro. inv MSTB. exploit mge_dom; eauto. intros [b2 X]. congruence.
     - exploit BC'INV; eauto. intros [(b'' & delta & J') | [A [B C]]].
       exploit Mem.loadbytes_inject. eexact Hm3. eauto. eauto. intros (bytes & A & B).
-      inv B. inv H6. inv H18. eapply PMTOP; eauto.
+      inv B. inv H6. inv H11. eapply PMTOP; eauto.
       eapply pmatch_incr; eauto.
       inv MM. exploit mmatch_top. eauto.
       intros [D E]. eapply E; eauto.
       erewrite Mem.loadbytes_unchanged_on_1 in H2; eauto.
-      intros. red. unfold compose_meminj, inj_of_bc.
+      intros. split. red. unfold compose_meminj, inj_of_bc.
       destruct (bc b); try congruence. rewrite B. reflexivity.
       rewrite B. reflexivity. rewrite B. reflexivity.
+      intro. inv MSTB. exploit mge_dom; eauto. intros [b2 X]. congruence.
   }
       econstructor; eauto.
       * (*sound_stack*)
         eapply sound_stack_new_bound.
-        2: inversion H11; eauto.
+        2: inversion H15; eauto.
         eapply sound_stack_exten.
         instantiate (1:= bc).
         eapply sound_stack_inv; eauto. intros.
         eapply Mem.loadbytes_unchanged_on_1; eauto.
-        intros. red. rewrite JBC_COMPOSE.
+        intros. split. red. rewrite JBC_COMPOSE.
         unfold jbc. rewrite H2. reflexivity.
+        intro. destruct GE0. exploit H8; eauto. intros [X Y]. congruence.
         intros.
         unfold bc'.  simpl. rewrite pred_dec_true; eauto.
       * (*romatch*)
@@ -1076,7 +1109,7 @@ Proof.
         -- apply SMTOP; auto.
         -- apply SMTOP; auto.
         -- red; simpl; intros. destruct (Mem.sup_dec b (Mem.support m)).
-           inv H11. eauto.
+           inv H15. eauto.
            destruct (j' b) as [[bx deltax] | ] eqn:J'.
            eapply Mem.valid_block_inject_1; eauto.
            congruence.
@@ -1104,7 +1137,7 @@ Theorem transf_program_correct prog tprog:
     (RTL.semantics prog) (RTL.semantics tprog).
 Proof.
   fsim (eapply Build_fsim_properties with (order := lt)
-                                          (match_states := fun i s1 s2 => match_states prog (snd w) i s1 s2
+                                          (match_states := fun i s1 s2 => match_states prog se1 se2 (snd w) i s1 s2
                                                                        /\ sound_state prog se1 s1
                                                                        /\ ro_mem (snd (fst w)) = m01 (snd w) )).
 - destruct w as [[se rw] w]. cbn in *. destruct Hse as [Hser Hse].
@@ -1117,9 +1150,10 @@ Proof.
 - destruct w as [[se [se' rwm]] w]. cbn in *. destruct Hse as [Hser Hse].
   inv Hser.
   intros q1' q2 s1 [q1 [Hqr Hq]] Hs1. inv Hqr. inv Hq. cbn in *. inv H2.
-  inv H. cbn in *. inv Hse. cbn in *. clear Hm Hm1.
+  inv H. cbn in *. inv Hse. cbn in *. clear Hm Hm1 gs0 gs3. rename gs4 into gs. rename gs5 into ge2.
   exploit transf_initial_states; eauto.
-  instantiate (2:= injpw f m1 m2 Hm0).
+  instantiate (1:= se2).
+  instantiate (1:= injpw f (Genv.genv_sup se) (Genv.genv_sup se2) m1 m2 Hm0).
   econstructor; eauto.
   eexists. split.
   econstructor; eauto. econstructor. eauto.
@@ -1129,7 +1163,7 @@ Proof.
 - destruct w as [[se [se' rwm]] w]. cbn in *. destruct Hse as [Hser Hse].
   inv Hser.
   intros n s1 s2 r1 (Hs & SOUND & M0) Hr1.
-  exploit transf_final_states; eauto. instantiate (1:= se).
+  exploit transf_final_states; eauto.
   intros [r2 [Hf [r3 [Ha Hb]]]].
   exists r2. split; eauto. exists r3. split; eauto. inv Ha.
   inv H. econstructor; eauto. constructor; eauto.
